thy/OpenFlow/OpenFlowDoc.thy
@@ -1,0 +1,20 @@
+section\<open>Conversion\<close>
+text{*
+All the results we present in this chapter are formalized and verified in Isabelle/HOL~\cite{nipkow2002isabelle}.
+This means that they can be trusted a level close to absolute certainty.
+*}
+theory OpenFlowDoc
+imports LinuxRouterOpenFlowTranslation
+begin
+subsection\<open>Linux Firewall Model\<close>
+subsubsection\<open>Routing Table\<close>
+subsubsection\<open>Firewall\<close>
+subsubsection\<open>Combined  and Simplified Model\<close>
+
+subsection\<open>OpenFlow Switch Model\<close>
+subsubsection\<open>Matching Flow Table entries\<close>
+subsubsection\<open>Evaluating a Flow Table\<close>
+
+subsection\<open>Conversion Implementation\<close>
+subsubsection\<open>Chaining Firewalls\<close>
+end
